checkpoint experimenting with mail server

src/Database/Proof/FilesysSpecsForMail.v
@@ -1,27 +1,125 @@
 From iris.proofmode Require Export tactics.
 From iris.algebra Require Import auth frac_auth.
+From iris.base_logic.lib Require Import invariants.
 
 From RecoveryRefinement Require Export CSL.WeakestPre CSL.Lifting.
 
 From RecoveryRefinement Require Import Database.Proof.BaseMachine.
+Require Import FilesysSpecs.
 
 Implicit Types (p:Path) (fh:Fd) (bs:ByteString).
 
 Definition path_dec : forall (a b : Path), {a=b}+{a<>b} := string_dec.
 
-Section lifting.
+Axiom is_tmpfile : Path -> bool.
+
+Section DerivedSpecs.
   Context `{!baseG Σ}.
   Context `{!inG Σ (authR (optionUR (exclR boolC)))}.
 
   (* TODO: should really be a set of paths, or invariant to permutation;
   currently ignoring this complication entirely *)
-  Definition dirents (G: gmap Path gname) : iProp Σ.
-  Admitted.
+  Definition direntsG (S: list Path) (G: gmap Path gname) : iProp Σ :=
+    ( dirents S ∗
+      ⌜ ∀ fn g, G !! fn = Some g -> is_tmpfile fn = true ⌝ ∗
+      ∀ fn g,
+        ⌜ G !! fn = Some g ⌝ -∗
+        own g (● (Excl' (if In_dec string_dec fn S then true else false))) )%I.
 
-  Theorem wp_create G p g :
-    {{{ ▷ (dirents G ∗ own g (◯ (Excl' false))) ∗ ⌜G !! p = Some g⌝ }}}
+  Definition dir_inv_inner (G: gmap Path gname) : iProp Σ :=
+    ( ∃ S,
+      direntsG S G ∗
+      ∀ fn, ⌜ fn ∈ S ⌝ -∗
+        if is_tmpfile fn then
+          True
+        else
+          ∃ bs, fn ↦ bs )%I.
+
+  Definition dirN : namespace := nroot .@ "dir".
+  Definition dir_inv (G : gmap Path gname) : iProp Σ :=
+    inv dirN (dir_inv_inner G).
+
+  Theorem create_ok G p g :
+    {{{ dir_inv G ∗ ▷ own g (◯ (Excl' false)) ∗ ⌜G !! p = Some g⌝ }}}
       FS.create p
-      {{{ fh, RET fh; dirents G ∗ own g (◯ (Excl' true)) ∗ p ↦ BS.empty ∗ fh ↦ (p, FS.Write) }}}.
+      {{{ fh, RET fh; own g (◯ (Excl' true)) ∗ p ↦ BS.empty ∗ fh ↦ (p, FS.Write) }}}.
+  Proof.
+    iIntros (phi).
+    iIntros "(#Hinv&Hown&#Heq) Post".
+
+    unfold dir_inv.
+    iInv dirN as (S) "(H1&H2)" "Hclose".
+
+    unfold direntsG.
+    iDestruct "H1" as "[Hx [#Hy Hz]]".
+
+    destruct (In_dec string_dec p S).
+    {
+      iSpecialize ("Hz" $! p g).
+      (* contradiction: Hown and Hz.  but the triangle is preventing us.. *)
+      (* iSpecialize ("Hy" with "Heq").
+         ...
+      *)
+    }
+
+    assert (¬ p ∈ S).
+    {
+      (* need some lemma about In implying elem_of *)
+      admit.
+    }
+
+    iApply (wp_create with "[Hx Heq]").
+    {
+      iNext.
+      iFrame.
+      eauto.
+    }
+
+    iNext.
+    iIntros (fh) "(Hdir&Hp&Hfd)".
+
+    iMod ("Hclose" with "[Hdir H2 Heq Hy Hz Hown]") as "_".
+    {
+      iNext.
+      iExists _.
+      unfold direntsG.
+      iSplitL "Hdir Hy Hz Hown". iSplitL "Hdir". iFrame.
+      {
+        iSplitL "Hy". eauto.
+        iIntros.
+        iSpecialize ("Hz" $! fn g0 a).
+        destruct (string_dec fn p).
+        {
+          subst.
+          rewrite a.
+          simpl; destruct (string_dec p p); try congruence.
+          (* g = g0 *)
+          (* p not in S *)
+          (* unify the two halves of the circles *)
+          admit.
+        }
+        {
+          (* fn != p, so equal to Hx *)
+          admit.
+        }
+      }
+
+      iIntros.
+      inversion a; subst.
+      {
+        iDestruct "Hy" as %?.
+        iDestruct "Heq" as %?.
+        specialize (H0 p g H1).
+        rewrite H0.
+        eauto.
+      }
+
+      iApply "H2". eauto.
+    }
+
+    iApply "Post".
+    iFrame.
+
   Admitted.
 
   Theorem wp_append fh bs' p bs :
@@ -39,9 +137,9 @@ Section lifting.
   (* TODO: is this the right spec? should [p ↦ bs] be in the precondition? how
   are [p ↦ ?] facts related to dirents S? *)
   Theorem wp_open G p bs :
-    {{{ ▷ (dirents G ∗ p ↦ bs) }}}
+    {{{ dir_inv G ∗ ▷ p ↦ bs }}}
       FS.open p
-      {{{ fh, RET fh; dirents G ∗ p ↦ bs ∗ fh ↦ (p, FS.Read) }}}.
+      {{{ fh, RET fh; p ↦ bs ∗ fh ↦ (p, FS.Read) }}}.
   Admitted.
 
   Theorem wp_readAt fh off len p bs :
@@ -57,26 +155,26 @@ Section lifting.
   Admitted.
 
   (* TODO: constrain result [r] in terms of owned ghost variables from g *)
-  Theorem wp_list G :
-    {{{ ▷ dirents G }}}
+  Theorem wp_list S G :
+    {{{ ▷ dirents S G }}}
       FS.list
-      {{{ r, RET r; dirents G }}}.
+      {{{ r, RET r; ⌜ r = S ⌝ }}}.
   Admitted.
 
   (* TODO: require no open FDs for the deleted file? *)
   Theorem wp_delete G p g bs :
-    {{{ ▷ (dirents G ∗ own g (◯ (Excl' true)) ∗ p ↦ bs) ∗ ⌜G !! p = Some g⌝ }}}
+    {{{ dir_inv G ∗ ▷ (own g (◯ (Excl' true)) ∗ p ↦ bs) ∗ ⌜G !! p = Some g⌝ }}}
       FS.delete p
-      {{{ RET (); dirents G ∗ own g (◯ (Excl' false)) }}}.
+      {{{ RET (); own g (◯ (Excl' false)) }}}.
   Admitted.
 
-  Theorem wp_link G (src dst : Path) g bs :
-    {{{ ▷ (dirents G ∗ src ↦ bs) }}}
+  Theorem wp_link G (src dst : Path) bs :
+    {{{ dir_inv G ∗ ▷ src ↦ bs }}}
       FS.link src dst
       {{{ ok, RET ok;
         match ok with
-        | false => dirents G ∗ src ↦ bs
-        | true => dirents G ∗ src ↦ bs ∗ dst ↦ bs ∗ own g (◯ (Excl' true)) ∗ ⌜G !! dst = Some g⌝
+        | false => src ↦ bs
+        | true => src ↦ bs ∗ dst ↦ bs (* XXX really need to connect to set of messages in mailbox *)
         end }}}.
   Admitted.
 
@@ -89,7 +187,6 @@ Section lifting.
 End lifting.
 
 (*
-Section DerivedSpecs.
   Context `{baseG Σ}.
 
   Local Open Scope bi_scope.
